ulib/FStar.ModifiesGen.fsti
@@ -780,10 +780,11 @@ val new_region_modifies
   (c: cls al)
   (m0: HS.mem)
   (r0: HS.rid)
+  (col: option int)
 : Lemma
-  (requires (HS.is_eternal_region r0 /\ HS.live_region m0 r0))
+  (requires (HS.is_eternal_region r0 /\ HS.live_region m0 r0 /\ (None? col \/ HS.is_eternal_color (Some?.v col))))
   (ensures (
-    let (_, m1) = HS.new_eternal_region m0 r0 None in
+    let (_, m1) = HS.new_eternal_region m0 r0 col in
     modifies (loc_none #_ #c) m0 m1
   ))
 
